

Chapter 9 Homework

Problem 1

Prove that for all integers n , k , and r for $r \leq k \leq n$ that

$$\binom{n}{k} \cdot \binom{k}{r} = \binom{n}{r} \cdot \binom{n-r}{k-r}$$

Proof

$$\begin{aligned}\binom{n}{k} \cdot \binom{k}{r} &= \frac{n!}{k!(n-k)!} \cdot \frac{k!}{r!(k-r)!} \text{ by definition of combinations} \\ &= \frac{n!k!}{k!(n-k)!r!(k-r)!} \text{ by multiplication} \\ &= \frac{n!}{(n-k)!r!(k-r)!} \text{ by canceling out } k! \\ &= \frac{n!}{r!(n-k)!(k-r)!} \text{ by commutative property} \\ &= \frac{n!(n-r)!}{r!(n-r)!(n-k)!(k-r)!} \text{ by multiplying by } 1 = \frac{(n-r)!}{(n-r)!} \\ &= \frac{n!}{r!(n-r)!} \cdot \frac{(n-r)!}{(k-r)!(n-k)!} \text{ by commutative property} \\ &= \frac{n!}{r!(n-r)!} \cdot \frac{(n-r)!}{(k-r)!(n-r-k+r)!} \text{ by adding } 0 = r-r \text{ to } (n-k)! \\ &= \frac{n!}{r!(n-r)!} \cdot \frac{(n-r)!}{(k-r)!(n-r-(k-r))!} \text{ by distributive property} \\ &= \binom{n}{r} \cdot \binom{n-r}{k-r} \text{ by definition of combination}\end{aligned}$$

Assuming that these integers are all positive, multiplying by $(n-r)!/(n-r)!$ works for $r \leq k \leq n$ because the recursive definition for factorial states that $0! = 1$.

Problem 1 Answer:

As shown in the proof above, by definition of equality

$$\binom{n}{k} \cdot \binom{k}{r} = \binom{n}{r} \cdot \binom{n-r}{k-r}$$

Problem 2

The binomial theorem states that for any real numbers a and b ,

$$(a + b)^n = \sum_{k=0}^n \binom{n}{k} a^{n-k} b^k \text{ for any integer } n \geq 0$$

Use this theorem to show that for any integer $n \geq 0$,

$$\sum_{k=0}^n (-1)^k \binom{n}{k} 3^{n-k} 2^k = 1$$

Proof

$$\begin{aligned} \sum_{k=0}^n (-1)^k \binom{n}{k} 3^{n-k} 2^k &= \sum_{k=0}^n \binom{n}{k} 3^{n-k} 2^k (-1)^k \text{ by commutative property} \\ &= \sum_{k=0}^n \binom{n}{k} 3^{n-k} (2 \cdot (-1))^k \text{ by distributive property} \\ &= \sum_{k=0}^n \binom{n}{k} 3^{n-k} (-2)^k \text{ by multiplication} \\ &= (3 - 2)^n \text{ by the binomial theorem} \\ &= 1^n \text{ by subtraction} \\ &= 1 \text{ because 1 to any power is 1} \end{aligned}$$

Problem 2 Answer:

As show in the proof above, by definition of equality

$$\sum_{k=0}^n (-1)^k \binom{n}{k} 3^{n-k} 2^k = 1$$